Adding k_spec to interp_prop_oom.

src/coq/Handlers/OOM.v
@@ -14,6 +14,7 @@ From Vellvm Require Import
      Utils.InterpPropOOM
      Utils.Error
      Utils.Tactics
+     Utils.InterpProp
      Semantics.LLVMEvents.
 
 From ITree Require Import
@@ -46,13 +47,13 @@ Ltac observe_vis :=
 
 Ltac observe_vis_r :=
   match goal with
-  | |- interp_prop_oomTF _ _ _ _ _ _ _ _ (VisF ?e ?k) =>
+  | |- interp_prop_oomTF _ _ _ _ _ _ _ _ _ (VisF ?e ?k) =>
       change (VisF e k) with (observe (Vis e k))
   end.
 
 Hint Constructors interp_prop_oomTF : INTERP_PROP_OOM.
 Hint Extern 1 (Vis _ _ ≅ Vis _ _) => reflexivity : INTERP_PROP_OOM.
-Hint Extern 5 (interp_prop_oomTF _ _ _ _ _ _ _
+Hint Extern 5 (interp_prop_oomTF _ _ _ _ _ _ _ _
                  _ (VisF _ _)) => observe_vis : INTERP_PROP_OOM.
 
 Ltac solve_interp_prop_oom :=
@@ -67,8 +68,31 @@ Section PARAMS_MODEL.
   Definition refine_OOM_handler : Effin ~> PropT Effout
     := fun _ e x => x ≈ trigger e.
 
+  Definition refine_OOM_k_spec
+    {T R : Type}
+    (e : Effin T)
+    (ta : itree Effout T)
+    (k2 : T -> itree Effout R)
+    (t2 : itree Effout R) : Prop
+    := eutt eq t2 (bind ta k2).
+
+  #[global] Instance k_spec_WF_refine_OOM_k_spec : k_spec_WF refine_OOM_handler (@refine_OOM_k_spec).
+  Proof.
+    split.
+    - intros A R2 e ta k2.
+      unfold Proper, respectful.
+      intros x y H.
+      unfold refine_OOM_k_spec.
+      rewrite H.
+      reflexivity.
+    - unfold refine_OOM_k_spec.
+      red.
+      intros T R2 e k2 t2 ta H H0.
+      auto.
+  Defined.
+
   Definition refine_OOM_h_flip {T} (RR : relation T) (target source : itree Effout T) : Prop
-    := @interp_prop_oom_l Effin Effout OOME _ _ refine_OOM_handler _ _ RR target source.
+    := @interp_prop_oom_l Effin Effout OOME _ _ refine_OOM_handler _ _ RR (@refine_OOM_k_spec) target source.
 
   Arguments refine_OOM_h_flip /.
 
@@ -109,7 +133,8 @@ Section PARAMS_MODEL.
         pstep. rewrite H0. econstructor; eauto. right. pclearbot.
         rewrite H0 in EQr.
         eapply CIH; eauto.
-        eapply interp_prop_oom_inv_tau; eauto; pstep; auto.
+        eapply interp_prop_oom_inv_tau; try typeclasses eauto.
+        eauto; pstep; auto.
       + pclearbot.
         inv EQr; try (exfalso; eapply EQ; eauto; fail).
         * clear CHECK.
@@ -125,25 +150,28 @@ Section PARAMS_MODEL.
              ++ rewrite itree_eta in HT1.
                 rewrite H1 in HT1.
                 pinversion HT1.
-             ++ red in H0. rewrite itree_eta in H1.
-                rewrite H3 in H1. rewrite H0 in H1.
-                setoid_rewrite bind_trigger in H1.
-                eapply eqit_inv in H1; inv H1.
+             ++ red in KS, HSPEC.
+                rewrite itree_eta in KS.
+                rewrite HSPEC in KS.
+                setoid_rewrite bind_trigger in KS.
+                rewrite H1 in KS.
+                eapply eqit_inv in KS; cbn in KS; inv KS.
           -- eapply IHHS0; eauto.
              assert (refine_OOM_h_flip RR t3 (Tau t1)) by (pstep; apply HS).
              eapply interp_prop_oom_inv_tau_r in H0; punfold H0.
+             typeclasses eauto.
           -- apply bisimulation_is_eq in HT1. rewrite HT1 in HS.
              cbn in HS. remember (VisF (subevent A e) k1).
              hinduction HS before CIH; intros; try (exfalso; eapply EQ; eauto; fail); inv Heqi; try discriminate.
              ++ constructor; eauto.
              ++ apply bisimulation_is_eq in HT1. rewrite HT1.
                 solve_interp_prop_oom.
-             ++ red in H0.
-                rewrite H0 in H1.
-                setoid_rewrite bind_trigger in H1.
-                rewrite itree_eta, H3 in H1.
-                punfold H1; red in H1; cbn in H1.
-                dependent induction H1.
+             ++ red in KS, HSPEC.
+                rewrite HSPEC in KS.
+                setoid_rewrite bind_trigger in KS.
+                rewrite itree_eta, H1 in KS.
+                punfold KS; red in KS; cbn in KS.
+                dependent induction KS.
                 unfold subevent in x.
                 unfold resum in x.
                 unfold ReSum_id in x.
@@ -153,34 +181,43 @@ Section PARAMS_MODEL.
                 observe_vis; solve_interp_prop_oom.                
           -- punfold HT1. red in HT1. cbn in HT1.
              dependent induction HT1.
-          -- red in H0. rewrite H0 in H1.
-             setoid_rewrite bind_trigger in H1.
-             remember (VisF e k1). rewrite itree_eta in H1.
+          -- red in HSPEC, KS. rewrite HSPEC in KS.
+             setoid_rewrite bind_trigger in KS.
+             remember (VisF e k1). rewrite itree_eta in KS.
              hinduction HS before CIH; intros; try (exfalso; eapply EQ; eauto; fail); try solve [inv Heqi]; solve_interp_prop_oom.
              ++ punfold HT1. red in HT1. cbn in HT1.
                 dependent induction HT1; repeat subst_existT.
-             ++ rewrite itree_eta in H1. rewrite Heqi in H1.
-                red in H0. rewrite H0 in H1. setoid_rewrite bind_trigger in H1.
-                apply eqit_inv in H1. cbn in H1. rewrite <- itree_eta in H3.
-                destruct H1 as (?&?&?); subst. cbn in H1.
-                unfold subevent in H1.
+             ++ red in KS.
+                rewrite itree_eta in KS. rewrite Heqi in KS.
+                red in HSPEC. rewrite HSPEC in KS. setoid_rewrite bind_trigger in KS.
+                apply eqit_inv in KS. cbn in KS. rewrite <- itree_eta in KS0.
+                destruct KS as (?&?&?); subst. cbn in *.
+                unfold subevent in KS0.
                 unfold subevent, resum, ReSum_id, id_, ReSum_inr, cat, Id_IFun, Cat_IFun, inr_,
-                  resum , ReSum_inl , cat, resum, Inr_sum1, inl_, Inl_sum1 in H1. inv H1.
-                eapply Interp_Prop_OomT_Vis. 3 : eauto. 2 : red; reflexivity. red in H3.
+                  resum , ReSum_inl , cat, resum, Inr_sum1, inl_, Inl_sum1 in KS0. inv H0.
+                eapply Interp_Prop_OomT_Vis. 3 : eauto. 2 : red; reflexivity.
 
-                setoid_rewrite H0 in HK. setoid_rewrite H2 in HK0.
+                setoid_rewrite HSPEC in HK.
                 intros; right; eapply CIH; pclearbot; eauto.
-                specialize (HK _ H1); pclearbot; eauto.
+                specialize (HK _ H0); pclearbot; eauto.
                 2: {
-                  rewrite H3.
+                  red.
+                  rewrite KS0.
                   setoid_rewrite bind_trigger.
                   reflexivity.
                 }
 
-                specialize (HK0 _ H1); pclearbot; eauto.
-                specialize (H4 a).
-                cbn in H4.
-                rewrite <- H4.
+                assert (Returns a ta0).
+                { rewrite HSPEC0.
+                  rewrite subevent_subevent.
+                  auto.
+                }
+                specialize (HK0 _ H3); pclearbot; eauto.
+                specialize (H1 a).
+                cbn in H1.
+                eapply interp_prop_oom_l_eutt_Proper; try typeclasses eauto.
+                rewrite <- H1; reflexivity.
+                reflexivity.
                 auto.
         * exfalso. rewrite itree_eta in HT1. rewrite H1 in HT1.
           apply eqit_inv in HT1; inv HT1.
@@ -201,22 +238,25 @@ Section PARAMS_MODEL.
       observe_vis; solve_interp_prop_oom.
     - (* oom right *)
       discriminate.
-    - rewrite itree_eta in H1.
+    - red in HSPEC, KS.
+      rewrite itree_eta in KS.
       hinduction EQr before z; intros; try inv Heqi; pclearbot.
-      + red in H0. rewrite H0 in H1. apply eqit_inv in H1; inv H1.
+      + rewrite HSPEC in KS. apply eqit_inv in KS; inv KS.
       + pstep; constructor; eauto.
-        red in H0. rewrite H0 in H1.
-        rewrite tau_eutt in H1. setoid_rewrite bind_vis in H1.
-        setoid_rewrite bind_ret_l in H1.
+        rewrite HSPEC in KS.
+        rewrite tau_eutt in KS. setoid_rewrite bind_vis in KS.
+        setoid_rewrite bind_ret_l in KS.
         assert (refine_OOM_h_flip RR t1 t0). do 2 red. apply HS.
-        unfold refine_OOM_h_flip in H2.
-        rewrite H1 in H2.
+        unfold refine_OOM_h_flip in *.
+        eapply interp_prop_oom_l_eutt_Proper in H0.
+        3: rewrite KS; reflexivity.
+        all: try reflexivity; try typeclasses eauto.
         clear HS.
-        punfold H2; red in H2; cbn in H2.
+        punfold H0; red in H0; cbn in H0.
         remember (VisF (subevent A e) (fun x : A => k2 x)).
-        hinduction H2 before z; intros; try inv Heqi; pclearbot.
+        hinduction H0 before z; intros; try inv Heqi; pclearbot.
         * constructor; auto; eapply IHinterp_prop_oomTF.
-        * rewrite itree_eta, H3 in HT1.
+        * rewrite itree_eta, H1 in HT1.
           punfold HT1; red in HT1; cbn in HT1.
           dependent induction HT1.
           unfold subevent, resum, ReSum_id, id_, ReSum_inr, cat, Id_IFun, Cat_IFun, inr_,
@@ -226,26 +266,25 @@ Section PARAMS_MODEL.
         * rewrite itree_eta in HT1.
           punfold HT1; red in HT1; cbn in HT1.
           dependent induction HT1.
-        * dependent destruction H6.
+        * dependent destruction H2.
           eapply Interp_Prop_OomT_Vis; eauto.
-          red in H2. rewrite H2 in H3. setoid_rewrite bind_trigger in H3.
+          red in KS0, HSPEC0. rewrite HSPEC0 in KS0. setoid_rewrite bind_trigger in KS0.
           intros. right; eapply CIH; eauto.
-          unfold subevent in H2.
+          unfold subevent in HSPEC0.
           unfold subevent, resum, ReSum_id, id_, ReSum_inr, cat, Id_IFun, Cat_IFun, inr_,
-            resum , ReSum_inl , cat, resum, Inr_sum1 in H2.
-          rewrite H2, <- H0 in H4.
-          specialize (HK _ H4); pclearbot. apply HK.
-          specialize (HK0 _ H4); pclearbot. apply HK0.
-      + eapply IHEQr. rewrite <- itree_eta. rewrite tau_eutt in H1; auto.
-      + specialize (IHEQr H1).
+            resum , ReSum_inl , cat, resum, Inr_sum1 in HSPEC0.
+          rewrite HSPEC0, <- HSPEC in H0.
+          specialize (HK _ H0); pclearbot. apply HK.
+          specialize (HK0 _ H0); pclearbot. apply HK0.
+      + eapply IHEQr. rewrite <- itree_eta. rewrite tau_eutt in KS; auto.
+      + specialize (IHEQr KS).
         pstep; constructor; auto. punfold IHEQr.
-      + red in H0.
-        rewrite H0 in H1.
-        rewrite HT1 in H1.
-        cbn in H1.
-        rewrite bind_trigger in H1.
-        punfold H1; red in H1; cbn in H1.
-        dependent induction H1.
+      + rewrite HSPEC in KS.
+        rewrite HT1 in KS.
+        cbn in KS.
+        rewrite bind_trigger in KS.
+        punfold KS; red in KS; cbn in KS.
+        dependent induction KS.
         unfold subevent, resum, ReSum_id, id_, ReSum_inr, cat, Id_IFun, Cat_IFun, inr_,
           resum , ReSum_inl , cat, resum, Inr_sum1 in x.
         inv x.
@@ -253,18 +292,22 @@ Section PARAMS_MODEL.
       + punfold HT1; red in HT1; cbn in HT1.
         dependent induction HT1.
       + pstep.
-        red in H0; rewrite H0 in H1; setoid_rewrite bind_trigger in H1.
-        apply eqit_inv in H1; cbn in H1.
-        destruct H1 as (?&?&?); subst. cbn in H1.
-        unfold subevent in H1.
+        rewrite HSPEC in KS; setoid_rewrite bind_trigger in KS.
+        apply eqit_inv in KS; cbn in KS.
+        destruct KS as (?&?&?); subst. cbn in *.
+        unfold subevent in H0.
         unfold subevent, resum, ReSum_id, id_, ReSum_inr, cat, Id_IFun, Cat_IFun, inr_,
-          resum , ReSum_inl , cat, resum, Inr_sum1, inl_, Inl_sum1 in H1. inv H1.
-        cbn in *. red in H2.
+          resum , ReSum_inl , cat, resum, Inr_sum1, inl_, Inl_sum1 in H0. inv H0.
+        cbn in *. red in HSPEC0, KS0.
         eapply Interp_Prop_OomT_Vis; eauto.
-        2 : rewrite <- itree_eta; eauto.
+        2 : red; rewrite <- itree_eta; eauto.
         intros. right. eapply CIH; eauto.
-        rewrite H2 in H1; setoid_rewrite H0 in HK; specialize (HK _ H1); pclearbot; eauto.
-        specialize (HK0 _ H1); pclearbot; rewrite <- H4; eauto.
+        rewrite HSPEC0 in H0; setoid_rewrite HSPEC in HK; specialize (HK _ H0); pclearbot; eauto.
+        specialize (HK0 _ H0); pclearbot.
+        eapply interp_prop_oom_l_eutt_Proper; try typeclasses eauto.
+        rewrite <- H1; reflexivity.
+        reflexivity.
+        eauto.
   Qed.
 
   #[global] Instance refine_OOM_h_reflexive {R} {RR : relation R} `{Reflexive _ RR} : Reflexive (refine_OOM_h RR).
@@ -280,6 +323,7 @@ Section PARAMS_MODEL.
 
     change (VisF e k2) with (observe (Vis e k2)).
     eapply Interp_Prop_OomT_Vis; eauto. red; reflexivity.
+    red.
     setoid_rewrite bind_trigger; reflexivity.
   Qed.
 
@@ -329,7 +373,7 @@ Proof.
   unfold Proper, respectful in H0.
 
   eapply H0; eauto.
-  typeclasses eauto.
+  all: try typeclasses eauto.
   apply eutt_flip; eauto.
   apply refine_OOM_h_reflexive; auto.
 Qed.
@@ -347,7 +391,10 @@ Proof.
 
   unfold raiseOOM.
   red.
+
+  eapply interp_prop_oom_l_eutt_Proper; try typeclasses eauto.
   rewrite bind_trigger.
+  all: try reflexivity.
 
   red.
   pstep; red; cbn.
@@ -361,12 +408,14 @@ Proof.
   intros x y XY z w ZW.
   split; intros REF; subst.
   - unfold refine_OOM_h, refine_OOM_h_flip in *.
-    rewrite ZW in REF.
-    rewrite XY in REF.
+    eapply interp_prop_oom_l_eutt_Proper; try typeclasses eauto.
+    rewrite <- ZW; reflexivity.
+    rewrite <- XY; reflexivity.
     auto.
   - unfold refine_OOM_h, refine_OOM_h_flip in *.
-    rewrite <- ZW in REF.
-    rewrite <- XY in REF.
+    eapply interp_prop_oom_l_eutt_Proper; try typeclasses eauto.
+    rewrite ZW; reflexivity.
+    rewrite XY; reflexivity.
     auto.
 Qed.
 
@@ -375,62 +424,63 @@ repeat intro. rewrite H, H0.
 reflexivity.
 Qed.
 
-Lemma refine_OOM_h_bind :
-  forall {T R E F} (x y : itree (E +' OOME +' F) T) (RR1 : relation T) (RR2 : relation R) k,
-    (forall r1 r2, RR1 r1 r2 -> refine_OOM_h RR2 (k r1) (k r2)) ->
-    refine_OOM_h RR1 x y ->
-    refine_OOM_h RR2 (a <- x;; k a) (a <- y;; k a).
-Proof.
-  intros T R E F.
+(* TODO: broken after k_spec changes *)
+(* Lemma refine_OOM_h_bind : *)
+(*   forall {T R E F} (x y : itree (E +' OOME +' F) T) (RR1 : relation T) (RR2 : relation R) k, *)
+(*     (forall r1 r2, RR1 r1 r2 -> refine_OOM_h RR2 (k r1) (k r2)) -> *)
+(*     refine_OOM_h RR1 x y -> *)
+(*     refine_OOM_h RR2 (a <- x;; k a) (a <- y;; k a). *)
+(* Proof. *)
+(*   intros T R E F. *)
 
-  unfold refine_OOM_h, refine_OOM_h_flip.
-  intros t1 t2 RR1 RR2.
+(*   unfold refine_OOM_h, refine_OOM_h_flip. *)
+(*   intros t1 t2 RR1 RR2. *)
 
-  unfold bind, Monad_itree.
-  revert t1 t2. pcofix CIH.
-  intros t1 t2 k HK EQT.
-  punfold EQT.
-  red in EQT.
+(*   unfold bind, Monad_itree. *)
+(*   revert t1 t2. pcofix CIH. *)
+(*   intros t1 t2 k HK EQT. *)
+(*   punfold EQT. *)
+(*   red in EQT. *)
 
-  assert (a <- t1 ;; k a =
-            match observe t1 with
-            | RetF r => k r
-            | TauF t0 => Tau (ITree.bind t0 k)
-            | @VisF _ _ _ X e ke => Vis e (fun x : X => ITree.bind (ke x) k)
-            end).
-  { apply bisimulation_is_eq; setoid_rewrite unfold_bind; reflexivity. }
-  setoid_rewrite H; clear H.
+(*   assert (a <- t1 ;; k a = *)
+(*             match observe t1 with *)
+(*             | RetF r => k r *)
+(*             | TauF t0 => Tau (ITree.bind t0 k) *)
+(*             | @VisF _ _ _ X e ke => Vis e (fun x : X => ITree.bind (ke x) k) *)
+(*             end). *)
+(*   { apply bisimulation_is_eq; setoid_rewrite unfold_bind; reflexivity. } *)
+(*   setoid_rewrite H; clear H. *)
 
-  assert (a <- t2 ;; k a =
-            match observe t2 with
-            | RetF r => k r
-            | TauF t0 => Tau (ITree.bind t0 k)
-            | @VisF _ _ _ X e ke => Vis e (fun x : X => ITree.bind (ke x) k)
-            end).
-  { apply bisimulation_is_eq; setoid_rewrite unfold_bind; reflexivity. }
-  setoid_rewrite H; clear H.
+(*   assert (a <- t2 ;; k a = *)
+(*             match observe t2 with *)
+(*             | RetF r => k r *)
+(*             | TauF t0 => Tau (ITree.bind t0 k) *)
+(*             | @VisF _ _ _ X e ke => Vis e (fun x : X => ITree.bind (ke x) k) *)
+(*             end). *)
+(*   { apply bisimulation_is_eq; setoid_rewrite unfold_bind; reflexivity. } *)
+(*   setoid_rewrite H; clear H. *)
 
-  pstep.
-  induction EQT; eauto; pclearbot; try discriminate.
-  - specialize (HK _ _ REL).
-    punfold HK.
-    eapply interp_prop_oomTF_mono. eapply HK.
-    intros. pclearbot. left.
-    eapply paco2_mon; eauto.
-    intros; contradiction.
-  - constructor. right.
-    eapply CIH; eauto.
-  - econstructor; auto.
-  - econstructor; auto.
-  - punfold HT1; red in HT1; cbn in HT1.
-    dependent induction HT1.
-    rewrite <- x.
-    red. solve_interp_prop_oom.
-  - eapply Interp_Prop_OomT_Vis; eauto.
-    intros; eauto. right. eapply CIH; eauto.
-    specialize (HK0 _ H1). pclearbot. eapply HK0; eauto.
-    rewrite <- unfold_bind.
-    setoid_rewrite <- Eqit.bind_bind.
-    eapply eutt_clo_bind; eauto. intros; eauto.
-    subst; reflexivity.
-Qed.
+(*   pstep. *)
+(*   induction EQT; eauto; pclearbot; try discriminate. *)
+(*   - specialize (HK _ _ REL). *)
+(*     punfold HK. *)
+(*     eapply interp_prop_oomTF_mono. eapply HK. *)
+(*     intros. pclearbot. left. *)
+(*     eapply paco2_mon; eauto. *)
+(*     intros; contradiction. *)
+(*   - constructor. right. *)
+(*     eapply CIH; eauto. *)
+(*   - econstructor; auto. *)
+(*   - econstructor; auto. *)
+(*   - punfold HT1; red in HT1; cbn in HT1. *)
+(*     dependent induction HT1. *)
+(*     rewrite <- x. *)
+(*     red. solve_interp_prop_oom. *)
+(*   - eapply Interp_Prop_OomT_Vis; eauto. *)
+(*     intros; eauto. right. eapply CIH; eauto. *)
+(*     specialize (HK0 _ H). pclearbot. eapply HK0; eauto. *)
+(*     rewrite <- unfold_bind. *)
+(*     setoid_rewrite <- Eqit.bind_bind. *)
+(*     eapply eutt_clo_bind; eauto. intros; eauto. *)
+(*     subst; reflexivity. *)
+(* Qed. *)
